@base <http://example.org/timonto/> .
@prefix rdf: <http://www.w3.org/1999/02/22-rdf-syntax-ns#> .
@prefix rdfs: <http://www.w3.org/2000/01/rdf-schema#> .
@prefix xsd: <http://www.w3.org/2001/XMLSchema#> .

#####################################################################################################
#																				                                                            #
#				                  Datatype properties	 						                                      		#
#								   		 										                                                          #
#####################################################################################################


<century>
	a			rdf:Property;
	rdfs:domain	<Century>;
	rdfs:range	xsd:positiveInteger.
	

<year>
	a			rdf:Property;
	rdfs:domain	<Year>;
	rdfs:range	xsd:gYear.
	
	
<leapYear>
	a			rdf:Property;
	rdfs:domain	<Year>;
	rdfs:range	xsd:boolean.
	
	
<month>
	a			rdf:Property;
	rdfs:domain	<MonthOfYear>;
	rdfs:range	xsd:gMonth.
	
	
<dayOfMonth>
	a			rdf:Property;
	rdfs:domain	<Day>;
	rdfs:range	xsd:gDay.
	
	
<numberOfDayOfMonth>
	a			rdf:Property;
	rdfs:domain	<MonthOfYear>;
	rdfs:range	xsd:positiveInteger.
	
	
<clockHour>
	a			rdf:Property;
	rdfs:domain	<Hour>;
	rdfs:range	xsd:positiveInteger.
	
	
<number>
	a			rdf:Property;
	rdfs:domain	<Date>;
	rdfs:range	xsd:positiveInteger;
	rdfs:comment	"Is used to have a modality of Date. For example when we want to use the <Date> 'first Saturday of June' ".


<last>
	a			rdf:Property;
	rdfs:domain	<Date>;
	rdfs:range	xsd:boolean;
	rdfs:comment	"Is used to have the last modality of Date. For example when we want to use the <Date> 'last Saturday of June' ".
	
	
<sample>
	a			rdf:Property;
	rdfs:domain	<Date>;
	rdfs:range	xsd:positiveInteger;
	rdfs:comment	"Is used to have a sample of Date. For example when we want to use the <Date> 'each three Saturday of June' ".
	
	
<even>
	a			rdf:Property;
	rdfs:domain	<Date>;
	rdfs:range	xsd:boolean;
	rdfs:comment	"Is used to specify the even parity of Date. If it is an odd date, even property is set to false".
	
	
<beginning>
	a			rdf:Property;
	rdfs:domain	<Date>;
	rdfs:range	xsd:boolean;
	rdfs:comment	"Is used to specify the beginning part of Date".
	
	
<middle>
	a			rdf:Property;
	rdfs:domain	<Date>;
	rdfs:range	xsd:boolean;
	rdfs:comment	"Is used to specify the middle part of Date".


<end>
	a			rdf:Property;
	rdfs:domain	<Date>;
	rdfs:range	xsd:boolean;
	rdfs:comment	"Is used to specify the end part of Date".
	

#####################################################################################################
#																		                                                            		#
#				                    Object Properties									                                      #
#																				                                                            #
#####################################################################################################
	
	
<hasMonth>
	a			rdf:Property;
	rdfs:domain	<Year>;
	rdfs:range	<Month>.
	
	
<hasDay>
	a			rdf:Property;
	rdfs:domain	<Month>;
	rdfs:range	<Day>.
	
	
<hasHour>
	a			rdf:Property;
	rdfs:domain	<Day>;
	rdfs:range	<Hour>.
	
	
<except>
	a			rdf:Property;
	rdfs:domain	<Every>;
	rdfs:range	<Date>;
	rdfs:comment	"""Used to specify exceptions within a non-convex interval""".		
	
	
<exp>
	a			rdf:Property;
	rdfs:domain	<Convex>, <Every>, <Period>;
	rdfs:range	<Thing>.
	
	
<atTime>
	a			rdf:Property;
	rdfs:domain	<Convex>, <Every>;
	rdfs:range	<Date>.
	
	
<before>
	a				rdf:Property;
	rdfs:domain		<Convex>, <Every>;
	rdfs:range		<Date>;
	rdfs:comment		"""To say one thing occur before a specific date""".
	

<list>
	a				rdf:Property;
	rdfs:subPropertyOf	rdfs:member;
	rdfs:subPropertyOf	<atTime>;
	rdfs:domain		<Enum>;
	rdfs:range		<Date>;
	rdfs:comment		"""Used to link an Enum date with these ordered values""".
	
	
<after>
	a				rdf:Property;
	rdfs:domain		<Convex>, <Every>;
	rdfs:range		<Date>;
	rdfs:comment		"""To say one thing occur after a specific date""".
	
	
<around>
	a				rdf:Property;
	rdfs:domain		<Convex>, <Every>;
	rdfs:range		<Date>;
	rdfs:comment		"""To say one thing occur around a specific date""".
	
	
<hasBegin>
	a				rdf:Property;
	rdfs:subPropertyOf	<atTime>;
	rdfs:domain		<During>;
	rdfs:range		<Date>;
	rdfs:comment		"""Used to specify the beginning of an interval between date units; a date unit is one year, one month, one day or one hour""".
					
					
<hasEnd>
	a				rdf:Property;
	rdfs:subPropertyOf	<atTime>;
	rdfs:domain		<During>;
	rdfs:range		<Date>;
	rdfs:comment		"""Used to specify the end of an interval between date units; a date unit is one year, one month, one day or one hour""".


<value>
	a				rdf:Property;
	rdfs:domain		<Thing>;
	rdfs:range		<Thing>.



#####################################################################################################
#																		                                                            		#
#				                   Classes										                                            	#
#																				                                                            #
#####################################################################################################

<Thing>
	a	rdfs:Class.


<Date> 	
	a				rdfs:Class;
	rdfs:subClassOf	<Thing>;	
	rdfs:comment		"Represents an abstract date which denotes different kind of date. It can be a simple date i.e. Century, Year, Month, so on or a regular date i.e. on September 2013, on 25 January 2014, so on ".
	
	
<Enum> 	
	a				rdfs:Class;
	rdfs:subClassOf	<Date>;
	rdfs:subClassOf	rdf:Seq; 	
	rdfs:comment		"Used to enumerate a list of ordered date".


<Century>
	a				rdfs:Class;
	rdfs:subClassOf	<Date>.
	

<Year>
	a				rdfs:Class;
	rdfs:subClassOf	<Date>.
	

<Week>
	a				rdfs:Class;
	rdfs:subClassOf	<Date>.
	
	
<Day>
	a				rdfs:Class;
	rdfs:subClassOf	<Date>.
	
	
<Hour>
	a				rdfs:Class;
	rdfs:subClassOf	<Date>.
	
	
<MonthOfYear>
	a				rdfs:Class;
	rdfs:subClassOf	<Date>.


<DayOfWeek>
	a				rdfs:Class;
	rdfs:subClassOf	<Day>.	

	
<GenericDay>
	a				rdfs:Class;
	rdfs:subClassOf	<Day>.


<TimeOfDay>
	a				rdfs:Class;
	rdfs:subClassOf	<Hour>.	
	

<Monday>
	a				rdfs:Class;
	rdfs:subClassOf	<DayOfWeek>.
	
	
<Tuesday>
	a				rdfs:Class;
	rdfs:subClassOf	<DayOfWeek>.
	
	
<Wednesday>
	a				rdfs:Class;
	rdfs:subClassOf	<DayOfWeek>.
	
	
<Thursday>
	a				rdfs:Class;
	rdfs:subClassOf	<DayOfWeek>.
	
	
<Friday>
	a				rdfs:Class;
	rdfs:subClassOf	<DayOfWeek>.
	
	
<Saturday>
	a				rdfs:Class;
	rdfs:subClassOf	<DayOfWeek>.
	
	
<Sunday>
	a				rdfs:Class;
	rdfs:subClassOf	<DayOfWeek>.
	
	
<Today>
	a				rdfs:Class;
	rdfs:subClassOf	<GenericDay>.
	
	
<Tomorrow>
	a				rdfs:Class;
	rdfs:subClassOf	<GenericDay>.
	
	
<Yesterday>
	a				rdfs:Class;
	rdfs:subClassOf	<GenericDay>.
	

	
<Morning>
	a				rdfs:Class;
	rdfs:subClassOf	<TimeOfDay>.
	
	
<Afternoon>
	a				rdfs:Class;
	rdfs:subClassOf	<TimeOfDay>.
	
	
<Evening>
	a				rdfs:Class;
	rdfs:subClassOf	<TimeOfDay>.
	
	
<Night>
	a				rdfs:Class;
	rdfs:subClassOf	<TimeOfDay>.
	
	
<Dawn>
	a				rdfs:Class;
	rdfs:subClassOf	<TimeOfDay>.
	
	
<Noon>
	a				rdfs:Class;
	rdfs:subClassOf	<TimeOfDay>.
	
	
<Dusk>
	a				rdfs:Class;
	rdfs:subClassOf	<TimeOfDay>.
	
	
<Midnight>
	a				rdfs:Class;
	rdfs:subClassOf	<TimeOfDay>.
	
	
<Period>
	a				rdfs:Class;
	rdfs:subClassOf	<Date>;
	rdfs:comment		"Cast Thing as a reference date".


<January>
	a				rdfs:Class;
	rdfs:subClassOf	<MonthOfYear>.
	

<February>
	a				rdfs:Class;
	rdfs:subClassOf	<MonthOfYear>.
	
	
<March>
	a				rdfs:Class;
	rdfs:subClassOf	<MonthOfYear>.
	
	
<April>
	a				rdfs:Class;
	rdfs:subClassOf	<MonthOfYear>.
	
	
<May>
	a				rdfs:Class;
	rdfs:subClassOf	<MonthOfYear>.
	
	
<June>
	a				rdfs:Class;
	rdfs:subClassOf	<MonthOfYear>.
	
	
<July>
	a				rdfs:Class;
	rdfs:subClassOf	<MonthOfYear>.
	
	
<August>
	a				rdfs:Class;
	rdfs:subClassOf	<MonthOfYear>.
	
	
<September>
	a				rdfs:Class;
	rdfs:subClassOf	<MonthOfYear>.
	
	
<October>
	a				rdfs:Class;
	rdfs:subClassOf	<MonthOfYear>.
	
	
<November>
	a				rdfs:Class;
	rdfs:subClassOf	<MonthOfYear>.
	
	
<December>
	a				rdfs:Class;
	rdfs:subClassOf	<MonthOfYear>.	


<Every>
	a				rdfs:Class;
	rdfs:subClassOf	<Thing>;
	rdfs:comment		"""Represents an interval with gaps (non-convex), i.e. a discontinuous interval""".


<Convex>
	a				rdfs:Class;
	rdfs:subClassOf	<Thing>;
	rdfs:comment		"""Represents an interval without gap, i.e. a continuous interval""".
	
	
<End>
	a				rdfs:Class;
	rdfs:subClassOf	<Convex>;
	rdfs:comment		"""Represents an open interval which one knows the end""".
	
	
<Start>
	a				rdfs:Class;
	rdfs:subClassOf	<Convex>;
	rdfs:comment		"""Represents an open interval which one knows the beginning""".
	
	
<During>
	a				rdfs:Class;
	rdfs:subClassOf	<Convex>;
	rdfs:comment		"""Represents a closed interval on one simple date; a simple date is a year, a month, a day or an hour""".
